Redefine cs as a function
This commit redefines cs as a function (rather than a relation), using
the optimal fixpoint combinator from LibFix. The new tactic cs_simpl is
used to simplify expressions involving cs.

This change somewhat simplified some proofs in CompleteSubstitutionFacts
(formerly SubstitutionFacts), but curiously made the proof in
Transitivity worse. Will have to investigate how it can be improved.

Substitution.v
@@ -13,19 +13,3 @@ Fixpoint subst (x : Var) (r : Sty) (orig : Sty) : Sty :=
   | var y => if beq_var x y then r else orig
   end
 .
-
-
-(* Read: cs S S' <=> cs S = S' *)
-Inductive cs : Sty -> Sty -> Prop :=
-| substall_unit : cs unit unit
-| substall_send : forall B S, cs (send B S) (send B S)
-| substall_recv : forall B S, cs (recv B S) (recv B S)
-| substall_echoice : forall S1 S2, cs (echoice S1 S2) (echoice S1 S2)
-| substall_ichoice : forall S1 S2, cs (ichoice S1 S2) (ichoice S1 S2)
-| substall_mu :
-    forall X S csS,
-    cs (subst X (mu X S) S) csS ->
-    cs (mu X S) csS
-| substall_var : forall X, cs (var X) (var X)
-.
-Hint Constructors cs : subst.
