CompleteSubstitution.v
@@ -1,0 +1,44 @@
+Require Import Env SessionTypes SessionTypesInd Substitution SubstitutionFacts
+  Tac TLC.LibFix Var Wellformed.
+
+Definition Cs cs S :=
+  match S with
+  | mu X S' => cs (subst X (mu X S') S')
+  | _       => S
+  end
+.
+
+Definition cs := FixFun Cs.
+
+Lemma cs_fix :
+  forall S,
+  ok_some S ->
+  cs S = Cs cs S.
+Proof.
+  applys (FixFun_fix_partial (lt_Sty_mu_prefix)).
+  - auto.
+  - unfolds. apply lt_Sty_mu_prefix_wf.
+  - unfolds. introv Hok H. destruct x; eauto with subst.
+Qed.
+
+
+Ltac cs_simpl :=
+  let ensure_constructor S :=
+    match S with
+    | unit => idtac
+    | send _ _ => idtac
+    | recv _ _ => idtac
+    | echoice _ _ => idtac
+    | ichoice _ _ => idtac
+    | mu _ _ => idtac
+    | var _ => idtac
+    end
+  with repl S :=
+    rewrite (cs_fix S) in *;
+    simpl (Cs cs S) in *
+  in
+  match goal with
+  | |- context [cs ?S] => ensure_constructor S; repl S
+  | H : context [cs ?S] |- _ => ensure_constructor S; repl S
+  end; [ try cs_simpl | eauto with subst wf .. ]
+.
