CompleteSubstitutionFacts.v
@@ -1,0 +1,142 @@
+Require Import CompleteSubstitution Equivalence SessionTypes SessionTypesInd
+  Shape ShapeFacts Substitution Tac Wellformed.
+
+Lemma cs_shape :
+  forall S,
+  ok_some S ->
+  shape (cs S) = unitS \/
+  shape (cs S) = sendS \/
+  shape (cs S) = recvS \/
+  shape (cs S) = ichoiceS \/
+  shape (cs S) = echoiceS.
+Proof.
+  induction S using (well_founded_ind lt_Sty_mu_prefix_wf); intros;
+    destruct S; cs_simpl; eauto with subst wf.
+Qed.
+
+
+Lemma cs_mu_absurd :
+  forall S X S',
+  ok_some S ->
+  cs S = mu X S' ->
+  False.
+Proof.
+  introv Hok H. eapply cs_shape in Hok. decompose_or_auto; shape_inv_auto;
+  discriminate.
+Qed.
+
+Hint Extern 1 =>
+  match goal with
+  | H : cs ?S1 = mu ?X1 ?S'1, Hok : ex ?XS1 (ok ?XS1 ?S1) |- _ =>
+      solve [ exfalso; exact (cs_mu_absurd S1 X1 S'1 Hok H) ]
+  end
+: subst.
+
+
+Lemma cs_preserves_sequiv :
+  forall S S',
+  ok_some S ->
+  ok_some  S' ->
+  sequiv S S' ->
+  sequiv (cs S) (cs S').
+Proof.
+  apply (
+    Sty_ind_mu_prefix2 (fun S S' =>
+      ok_some S ->
+      ok_some S' ->
+      sequiv S S' ->
+      sequiv (cs S) (cs S'))
+  ).
+  introv IH Hok Hok' Heq. inverts2 Heq; cs_simpl; eauto 10 with subst.
+Qed.
+
+
+Lemma uncs_preserves_sequiv_l :
+  forall S S',
+  ok_some S ->
+  sequiv (cs S) S' ->
+  sequiv S S'.
+Proof.
+  induction S using (well_founded_ind lt_Sty_mu_prefix_wf);
+    intros; destruct S; cs_simpl; eauto 10 with subst.
+Qed.
+
+
+Lemma uncs_preserves_sequiv_r :
+  forall S S',
+  ok_some S' ->
+  sequiv S (cs S') ->
+  sequiv S S'.
+Proof.
+  induction S' using (well_founded_ind lt_Sty_mu_prefix_wf);
+    intros; destruct S'; cs_simpl; eauto 10 with subst.
+Qed.
+
+
+Lemma uncs_preserves_sequiv :
+  forall S S',
+  ok_some S ->
+  ok_some S' ->
+  sequiv (cs S) (cs S') ->
+  sequiv S S'.
+Proof.
+  intros. eapply uncs_preserves_sequiv_l; eauto.
+  eapply uncs_preserves_sequiv_r; eauto.
+Qed.
+
+
+Lemma cs_preserves_sequiv_l :
+  forall S S',
+  ok_some S ->
+  ok_some S' ->
+  sequiv S S' ->
+  sequiv (cs S) S'.
+Proof.
+  intros. eapply uncs_preserves_sequiv_r; eauto.
+  eapply cs_preserves_sequiv; eauto.
+Qed.
+
+
+Lemma cs_preserves_sequiv_r :
+  forall S S',
+  ok_some S ->
+  ok_some S' ->
+  sequiv S S' ->
+  sequiv S (cs S').
+Proof.
+  intros. eapply uncs_preserves_sequiv_l; eauto.
+  eapply cs_preserves_sequiv; eauto.
+Qed.
+
+
+Lemma cs_preserves_not_sequiv :
+  forall S S',
+  ok_some S ->
+  ok_some S' ->
+  ~ sequiv S S' ->
+  ~ sequiv (cs S) (cs S').
+Proof.
+  introv Hok Hok' H contra. apply H. eapply uncs_preserves_sequiv; eauto.
+Qed.
+
+
+Lemma uncs_preserves_not_sequiv :
+  forall S S',
+  ok_some S ->
+  ok_some S' ->
+  ~ sequiv (cs S) (cs S') ->
+  ~ sequiv S S'.
+Proof.
+  introv Hok Hok' H contra. apply H. eapply cs_preserves_sequiv; eauto.
+Qed.
+
+
+Lemma cs_preserves_wellformedness :
+  forall S,
+  wellformed S ->
+  wellformed (cs S).
+Proof.
+  induction S using (well_founded_ind lt_Sty_mu_prefix_wf);
+    introv Hwf; destruct S; cs_simpl; eauto 10 with subst.
+Qed.
+Hint Resolve cs_preserves_wellformedness : subst.
