Transitivity.v
@@ -1,5 +1,6 @@
-Require Import Equivalence Reflexivity SessionTypes SessionTypesInd
-  Substitution SubstitutionFacts Tac Wellformed.
+Require Import CompleteSubstitution CompleteSubstitutionFacts Equivalence
+  Reflexivity SessionTypes SessionTypesInd Substitution SubstitutionFacts
+  Tac Wellformed.
 
 Create HintDb trans discriminated.
 Hint Resolve sequiv_reflexive : trans.
@@ -62,92 +63,97 @@ Proof.
 
   apply trans_helper_transitive. apply sequiv_coind.
   introv H. rename S' into U. inverts H.
-  assert (exists csT, cs T csT) as HcsT by eauto using cs_ex.
-  decompose_ex_auto.
-  assert (sequiv S csT) as HSeqT by (
-    eapply cs_preserves_sequiv_r with (S := S) (S' := T);
-    eauto using cs_preserves_sequiv_l
+  assert (sequiv S (cs T)) as HSeqT by (
+    eapply cs_preserves_sequiv_r; eauto with subst
   ).
-  assert (sequiv csT U) as HTeqU by (
-    eapply cs_preserves_sequiv_l with (S := T) (S' := U);
-    eauto using cs_preserves_sequiv_r
+  assert (sequiv (cs T) U) as HTeqU by (
+    eapply cs_preserves_sequiv_l; eauto with subst
   ).
-  clear H3 H4. inverts2 HSeqT; inverts2 HTeqU.
+  clear H3 H4. inverts2 HSeqT; inverts2 HTeqU; subst; try solve [false].
 
   (* unit *)
   - auto.
 
-  - constructor. apply sequiv_impl_trans_helper; auto.
+  - constructor. rewrite <- HSeqT in *.
+    apply sequiv_impl_trans_helper; auto with wf.
 
   (* send *)
-  - constructor. apply trans_helper_trans with (T := S'); eauto with wf.
-      assert (wellformed (send B S')) by
-        (eapply cs_preserves_wellformedness; eauto with wf).
+  - rewrite <- H4 in H3. injection H3; intros; subst.
+    constructor. apply trans_helper_trans with (T := S); eauto with wf.
+      apply cs_preserves_wellformedness in H1. rewrite <- H4 in H1.
       eauto with wf.
 
-  - constructor. apply trans_helper_trans with (T := send B S'); eauto with wf.
-      eapply cs_preserves_wellformedness; eauto with wf.
+  - constructor. rewrite <- H3 in *.
+    apply trans_helper_trans with (T := send B S'); eauto with wf.
+      rewrite H3. eapply cs_preserves_wellformedness; eauto with wf.
 
   (* recv *)
-  - constructor. apply trans_helper_trans with (T := S'); eauto with wf.
-      assert (wellformed (recv B S')) by
-        (eapply cs_preserves_wellformedness; eauto with wf).
+  - rewrite <- H4 in H3. injection H3; intros; subst.
+    constructor. apply trans_helper_trans with (T := S); eauto with wf.
+      apply cs_preserves_wellformedness in H1. rewrite <- H4 in H1.
       eauto with wf.
 
-  - constructor. apply trans_helper_trans with (T := recv B S'); eauto with wf.
-      eapply cs_preserves_wellformedness; eauto with wf.
+  - constructor. rewrite <- H3 in *.
+    apply trans_helper_trans with (T := recv B S'); eauto with wf.
+      rewrite H3. eapply cs_preserves_wellformedness; eauto with wf.
 
   (* echoice *)
   - assert (wellformed (echoice S1' S2')) by
-      (eapply cs_preserves_wellformedness; eauto with wf).
+      (rewrite H3; eapply cs_preserves_wellformedness; eauto with wf).
+    rewrite <- H4 in H3. injection H3; intros; subst.
     constructor.
-    * apply trans_helper_trans with (T := S1'); eauto with wf.
-    * apply trans_helper_trans with (T := S2'); eauto with wf.
+    * apply trans_helper_trans with (T := S0); eauto with wf.
+    * apply trans_helper_trans with (T := S3); eauto with wf.
 
   - assert (wellformed (echoice S1' S2')) by
-      (eapply cs_preserves_wellformedness; eauto with wf).
-    constructor. apply trans_helper_trans with (T := echoice S1' S2');
-      eauto with wf.
+      (rewrite H3; eapply cs_preserves_wellformedness; eauto with wf).
+    constructor. rewrite <- H3 in *.
+    apply trans_helper_trans with (T := echoice S1' S2'); eauto with wf.
 
   (* ichoice *)
   - assert (wellformed (ichoice S1' S2')) by
-      (eapply cs_preserves_wellformedness; eauto with wf).
+      (rewrite H3; eapply cs_preserves_wellformedness; eauto with wf).
+    rewrite <- H4 in H3. injection H3; intros; subst.
     constructor.
-    * apply trans_helper_trans with (T := S1'); eauto with wf.
-    * apply trans_helper_trans with (T := S2'); eauto with wf.
+    * apply trans_helper_trans with (T := S0); eauto with wf.
+    * apply trans_helper_trans with (T := S3); eauto with wf.
 
   - assert (wellformed (ichoice S1' S2')) by
-      (eapply cs_preserves_wellformedness; eauto with wf).
-    constructor. apply trans_helper_trans with (T := ichoice S1' S2');
-      eauto with wf.
+      (rewrite H3; eapply cs_preserves_wellformedness; eauto with wf).
+    constructor. rewrite <- H3 in *.
+    apply trans_helper_trans with (T := ichoice S1' S2'); eauto with wf.
 
   (* unit *)
-  - constructor. apply sequiv_impl_trans_helper; auto.
+  - rewrite <- HTeqU in *. constructor. apply sequiv_impl_trans_helper; auto.
 
   (* send *)
-  - constructor. apply trans_helper_trans with (T := send B S); auto.
-      eauto using cs_preserves_wellformedness with wf.
+  - constructor. rewrite <- H3 in *.
+    apply trans_helper_trans with (T := send B S); auto.
+      rewrite H3; eauto using cs_preserves_wellformedness with wf.
 
   (* recv *)
-  - constructor. apply trans_helper_trans with (T := recv B S); auto.
-      eauto using cs_preserves_wellformedness with wf.
+  - constructor. rewrite <- H3 in *.
+    apply trans_helper_trans with (T := recv B S); auto.
+      rewrite H3; eauto using cs_preserves_wellformedness with wf.
 
   (* echoice *)
-  - constructor. apply trans_helper_trans with (T := echoice S1 S2); auto.
-      eauto using cs_preserves_wellformedness with wf.
+  - constructor. rewrite <- H3 in *.
+    apply trans_helper_trans with (T := echoice S1 S2); auto.
+      rewrite H3; eauto using cs_preserves_wellformedness with wf.
 
   (* ichoice *)
-  - constructor. apply trans_helper_trans with (T := ichoice S1 S2); auto.
-      eauto using cs_preserves_wellformedness with wf.
+  - constructor. rewrite <- H3 in *.
+    apply trans_helper_trans with (T := ichoice S1 S2); auto.
+      rewrite H3; eauto using cs_preserves_wellformedness with wf.
 
   (* mu 1 (impossible) *)
   - exfalso; eauto using cs_mu_absurd.
 
   (* mu 2 *)
   - constructor.
-    assert (sequiv csT (mu X0 S')) as HTeqU' by auto.
-    apply trans_helper_trans with (T := csT); eauto with wf.
-      eauto using cs_preserves_wellformedness.
+    assert (sequiv (cs T) (mu X0 S')) as HTeqU' by auto.
+    apply trans_helper_trans with (T := cs T);
+      eauto using cs_preserves_wellformedness with wf.
 
   (* mu 3 (impossible) *)
   - exfalso; eauto using cs_mu_absurd.
